proofs/x86-64/avx2/ml_dsa_65/hashing.ec
@@ -17,6 +17,7 @@ from CryptoSpecs require import JWordList.
 (****************************************************************************)
 
 from Keccak require import Keccak1600_avx2.
+from Keccak require import Keccakf1600_avx2.
 
 equiv state_init_avx2_eq:
  M.__state_init_avx2 ~ Keccak1600_Jazz.M.__state_init_avx2
@@ -399,8 +400,11 @@ qed.
 equiv derive_commitment_hash_eq:
  M.__derive_commitment_hash ~ K.__derive_commitment_hash
  : ={arg} ==> ={res}.
-  proc.  admit.
-(* by inline *;sim; auto => />. *)
+proc. 
+seq 4 4 : (={encoded_commitment,state,commitment_hash}); 1: by inline *;sim.
+seq 1 1 : (={encoded_commitment,state,commitment_hash}); 2: by inline *;sim.
+inline {1} 1; inline {2} 1.
+by sim; auto => />.
 qed.
 
 equiv derive_message_representative_eq:
@@ -412,59 +416,302 @@ equiv derive_message_representative_eq:
 (* Correctness lemmas (absorbed-state characterization)                     *)
 (****************************************************************************)
 
+hoare shake256_absorb_34_h' _seed _extra :
+ K.shake256_absorb_34
+ : arg.`1 = _seed /\ arg.`2 = _extra
+ ==> res = stavx2_from_st25 (keccak_f1600_op (ABSORB1600 (W8.of_int 31) 136 (to_list _seed ++ to_list _extra))).
+proof.
+proc.
+ecall (keccakf1600_avx2_h (stavx2_to_st25 state)).
+wp; ecall (A2avx2.absorb_avx2_h (to_list seed) extra 31 136).
+wp; ecall (A32avx2.absorb_avx2_h [<:W8.t>] seed 0 136).
+wp; call (state_init_avx2_h 136).
+auto => |> st0 ? [st1 x2] ??; split; 1: by smt(Array32.size_to_list).
+move => ? [st2 x3] /= -> /=; split; 1: by rewrite /absorb_spec_avx2  stavx2_from_st25K.
+by move => ->; rewrite !stavx2_from_st25K.
+qed.
+
+lemma shake256_absorb_34_ll: islossless K.shake256_absorb_34.
+proof.
+proc.
+call keccakf1600_avx2_ll.
+call A2avx2.absorb_avx2_ll.
+call A32avx2.absorb_avx2_ll.
+call state_init_avx2_ll.
+by auto.
+qed.
+
+phoare shake256_absorb_34_ph' _seed _extra :
+ [ K.shake256_absorb_34
+ : arg.`1 = _seed /\ arg.`2 = _extra
+ ==> res = stavx2_from_st25 (keccak_f1600_op (ABSORB1600 (W8.of_int 31) 136 (to_list _seed ++ to_list _extra)))
+ ] = 1%r.
+proof.
+by conseq shake256_absorb_34_ll (shake256_absorb_34_h' _seed _extra).
+qed.
+
 phoare shake256_absorb_34_ph _seed _extra :
  [ M.shake256_absorb_34
  : arg.`1 = _seed /\ arg.`2 = _extra
- ==> absorb_spec_avx2 136 31 (to_list _seed ++ to_list _extra) res
+ ==> res = stavx2_from_st25 (keccak_f1600_op (ABSORB1600 (W8.of_int 31) 136 (to_list _seed ++ to_list _extra)))
  ] = 1%r.
-admitted.
+proof.
+by conseq shake256_absorb_34_eq (shake256_absorb_34_ph' _seed _extra) => // /#.
+qed.
+
+(* ---------- shake256_absorb_66 ---------- *)
+
+hoare shake256_absorb_66_h' _rho_prime _ds :
+ K.shake256_absorb_66
+ : arg.`1 = _rho_prime /\ arg.`2 = _ds
+ ==> res = stavx2_from_st25 (keccak_f1600_op (ABSORB1600 (W8.of_int 31) 136
+      (to_list _rho_prime ++ to_list _ds))).
+proof.
+proc.
+ecall (keccakf1600_avx2_h (stavx2_to_st25 state)).
+wp; ecall (A2avx2.absorb_avx2_h (to_list rho_prime) ds 31 136).
+wp.
+ecall (A64avx2.absorb_avx2_h [<:W8.t>] rho_prime 0 136).
+wp; call (state_init_avx2_h 136).
+auto => |> st0 ? [st1 x2] ??; split; 1: by smt(Array64.size_to_list).
+move => ? [st2 x3] /= -> /=; split; 1: by rewrite /absorb_spec_avx2 stavx2_from_st25K.
+move => ->; rewrite !stavx2_from_st25K /=;do !congr.
+apply (eq_from_nth witness); 1: by rewrite size_to_list /=.
+move => i; rewrite size_to_list /= => ib.
+by rewrite initiE 1:/# get8_set16_directE //= /#.
+qed.
+
+lemma shake256_absorb_66_ll: islossless K.shake256_absorb_66.
+proof.
+proc.
+call keccakf1600_avx2_ll.
+call A2avx2.absorb_avx2_ll.
+wp.
+call A64avx2.absorb_avx2_ll.
+call state_init_avx2_ll.
+by auto.
+qed.
+
+phoare shake256_absorb_66_ph' _rho_prime _ds :
+ [ K.shake256_absorb_66
+ : arg.`1 = _rho_prime /\ arg.`2 = _ds
+ ==> res = stavx2_from_st25 (keccak_f1600_op (ABSORB1600 (W8.of_int 31) 136
+      (to_list _rho_prime ++ to_list _ds)))
+ ] = 1%r.
+proof.
+by conseq shake256_absorb_66_ll (shake256_absorb_66_h' _rho_prime _ds).
+qed.
 
 phoare shake256_absorb_66_ph _rho_prime _ds :
  [ M.shake256_absorb_66
  : arg.`1 = _rho_prime /\ arg.`2 = _ds
- ==> absorb_spec_avx2 136 31
-      (to_list _rho_prime ++
-       to_list (Array2.init (WArray2.get8 (WArray2.set16 (WArray2.init8 (fun i => witness)) 0 _ds))))
-      res
+ ==> res = stavx2_from_st25 (keccak_f1600_op (ABSORB1600 (W8.of_int 31) 136
+      (to_list _rho_prime ++ to_list _ds)))
  ] = 1%r.
-admitted.
+proof.
+by conseq shake256_absorb_66_eq (shake256_absorb_66_ph' _rho_prime _ds) => // /#.
+qed.
+
+(* ---------- shake256_absorb_128 ---------- *)
+
+hoare shake256_absorb_128_h' _block :
+ K.shake256_absorb_128
+ : arg = _block
+ ==> res = stavx2_from_st25 (keccak_f1600_op (ABSORB1600 (W8.of_int 31) 136 (to_list _block))).
+proof.
+proc.
+ecall (keccakf1600_avx2_h (stavx2_to_st25 state)).
+wp; ecall (A128avx2.absorb_avx2_h [<:W8.t>] block 31 136).
+wp; call (state_init_avx2_h 136).
+auto => |> st0 ? [st1 x2]; rewrite /absorb_spec_avx2  => H; split; 1: by rewrite stavx2_to_st25K /=; smt( stavx2INV_from_st25).
+by move => /= ->; rewrite H !stavx2_from_st25K.
+qed.
+
+lemma shake256_absorb_128_ll: islossless K.shake256_absorb_128.
+proof.
+proc.
+call keccakf1600_avx2_ll.
+call A128avx2.absorb_avx2_ll.
+call state_init_avx2_ll.
+by auto.
+qed.
+
+phoare shake256_absorb_128_ph' _block :
+ [ K.shake256_absorb_128
+ : arg = _block
+ ==> res = stavx2_from_st25 (keccak_f1600_op (ABSORB1600 (W8.of_int 31) 136 (to_list _block)))
+ ] = 1%r.
+proof.
+by conseq shake256_absorb_128_ll (shake256_absorb_128_h' _block).
+qed.
 
 phoare shake256_absorb_128_ph _block :
  [ M.shake256_absorb_128
  : arg = _block
- ==> absorb_spec_avx2 136 31 (to_list _block) res
+ ==> res = stavx2_from_st25 (keccak_f1600_op (ABSORB1600 (W8.of_int 31) 136 (to_list _block)))
  ] = 1%r.
-admitted.
+proof.
+by conseq shake256_absorb_128_eq (shake256_absorb_128_ph' _block) => // /#.
+qed.
+
+(* ---------- shake256_absorb_commitment_hash ---------- *)
+
+hoare shake256_absorb_commitment_hash_h' _hash :
+ K.shake256_absorb_commitment_hash
+ : arg = _hash
+ ==> res = stavx2_from_st25 (keccak_f1600_op (ABSORB1600 (W8.of_int 31) 136 (to_list _hash))).
+proof.
+proc.
+ecall (keccakf1600_avx2_h (stavx2_to_st25 state)).
+wp; ecall (A48avx2.absorb_avx2_h [<:W8.t>] hash 31 136).
+wp; call (state_init_avx2_h 136).
+auto => |> st0 ? [st1 x2]; rewrite /absorb_spec_avx2 => H; split; 1: by rewrite stavx2_to_st25K /=; smt(stavx2INV_from_st25).
+by move => /= ->; rewrite H !stavx2_from_st25K.
+qed.
+
+lemma shake256_absorb_commitment_hash_ll: islossless K.shake256_absorb_commitment_hash.
+proof.
+proc.
+call keccakf1600_avx2_ll.
+call A48avx2.absorb_avx2_ll.
+call state_init_avx2_ll.
+by auto.
+qed.
+
+phoare shake256_absorb_commitment_hash_ph' _hash :
+ [ K.shake256_absorb_commitment_hash
+ : arg = _hash
+ ==> res = stavx2_from_st25 (keccak_f1600_op (ABSORB1600 (W8.of_int 31) 136 (to_list _hash)))
+ ] = 1%r.
+proof.
+by conseq shake256_absorb_commitment_hash_ll (shake256_absorb_commitment_hash_h' _hash).
+qed.
 
 phoare shake256_absorb_commitment_hash_ph _hash :
  [ M.shake256_absorb_commitment_hash
  : arg = _hash
- ==> absorb_spec_avx2 136 31 (to_list _hash) res
+ ==> res = stavx2_from_st25 (keccak_f1600_op (ABSORB1600 (W8.of_int 31) 136 (to_list _hash)))
  ] = 1%r.
-admitted.
+proof.
+by conseq shake256_absorb_commitment_hash_eq (shake256_absorb_commitment_hash_ph' _hash) => // /#.
+qed.
 
 (****************************************************************************)
 (* Correctness lemmas (complete hash operations)                            *)
 (****************************************************************************)
+require import Mldsa_65_prelude.
+hoare hash_verification_key_h' _vk :
+ K.hash_verification_key
+ : arg.`2 = _vk
+ ==> res = Array64.of_list witness (Bytes64.to_list (H_tr (BytesPK.of_list (to_list _vk)))).
+proof.
+proc.
+ecall (A64avx2.dumpstate_avx2_h verification_key_hash 0 64 state).
+ecall (keccakf1600_avx2_h (stavx2_to_st25 state)).
+wp; ecall (A1952avx2.absorb_avx2_h [<:W8.t>] verification_key 31 136).
+wp; call (state_init_avx2_h 136).
+auto => |> &hr st0 ? [st1 x1]; rewrite /absorb_spec_avx2 => Hab; split.
++ by rewrite stavx2_to_st25K; smt(stavx2INV_from_st25).
+move => -> [rr1 rr2] /= -> ?.
+rewrite Hab !stavx2_from_st25K.
+apply Array64.tP => i Hi /=.
+rewrite Array64.get_of_list 1://.
+rewrite Bytes64.get_to_list /H_tr.
+rewrite Bytes64.get_of_list 1://.
+rewrite BytesPK.of_listK 1:Array1952.size_to_list; 1: by rewrite mldsa65_kvec /=.
+rewrite /SHAKE256 /KECCAK1600 /SQUEEZE1600 /squeezeblocks /squeezestate_i /st_i /squeezestate /SHAKE_DS_BYTE /c512_r8.
+have -> : (64 - 1) %/ 136 + 1 = 1 by done.
+rewrite -iotaredE /= fillE initiE 1:/# /= Hi /= nth_take 1,2:/# flatten1 nth_take 1,2:/#.
+rewrite iter1 /= (nth_change_dfl W8.zero witness); 1: by rewrite size_state2bytes /= /#.
+by rewrite state2bytesE. 
+qed.
+
+lemma hash_verification_key_ll : islossless K.hash_verification_key.
+proof.
+proc.
+call A64avx2.dumpstate_avx2_ll.
+call keccakf1600_avx2_ll.
+call A1952avx2.absorb_avx2_ll.
+call state_init_avx2_ll.
+by auto.
+qed.
+
+phoare hash_verification_key_ph' _vk :
+ [ K.hash_verification_key
+ : arg.`2 = _vk
+ ==> res = Array64.of_list witness (Bytes64.to_list (H_tr (BytesPK.of_list (to_list _vk))))
+ ] = 1%r.
+proof.
+by conseq hash_verification_key_ll (hash_verification_key_h' _vk).
+qed.
 
 phoare hash_verification_key_correct _vk :
  [ M.hash_verification_key
  : arg.`2 = _vk
  ==> res = Array64.of_list witness (Bytes64.to_list (H_tr (BytesPK.of_list (to_list _vk))))
  ] = 1%r.
-admitted.
+proof.
+by conseq hash_verification_key_eq (hash_verification_key_ph' _vk) => // /#.
+qed.
+
+hoare derive_commitment_hash_h' _mu _w1 :
+ K.__derive_commitment_hash
+ : arg.`1 = _mu /\ arg.`2 = _w1
+ ==> res = Array48.of_list witness (BytesCT.to_list (H_ct (Bytes64.of_list (to_list _mu)) (BytesW1.of_list (to_list _w1)))).
+proof.
+proc.
+ecall (A48avx2.dumpstate_avx2_h commitment_hash 0 48 state).
+ecall (keccakf1600_avx2_h (stavx2_to_st25 state)).
+wp; ecall (A768avx2.absorb_avx2_h (to_list message_representative) encoded_commitment 31 136).
+wp; ecall (A64avx2.absorb_avx2_h [<:W8.t>] message_representative 0 136).
+wp; call (state_init_avx2_h 136).
+auto => |> st0 ? [st1 x1] ??; split; 1: by smt(Array64.size_to_list).
+move => ? [st2 x2]; rewrite /absorb_spec_avx2 => Hab; split.
++ by rewrite stavx2_to_st25K; smt(stavx2INV_from_st25).
+move => -> [rr1 rr2] /= -> ?.
+rewrite Hab !stavx2_from_st25K.
+apply Array48.tP => i Hi /=.
+rewrite Array48.get_of_list 1://.
+rewrite BytesCT.get_to_list /H_ct.
+rewrite BytesCT.get_of_list 1:// mldsa65_lambda 1:/#.
+rewrite Bytes64.of_listK 1:Array64.size_to_list // BytesW1.of_listK 1:Array768.size_to_list; 1: by  rewrite mldsa65_kvec.
+rewrite /SHAKE256 /KECCAK1600 /SQUEEZE1600 /squeezeblocks /squeezestate_i /st_i /squeezestate /SHAKE_DS_BYTE /c512_r8.
+have -> : (48 - 1) %/ 136 + 1 = 1 by done.
+rewrite -iotaredE /= fillE initiE 1:/# /= Hi /= nth_take 1,2:/# flatten1 nth_take 1,2:/#.
+rewrite iter1 /= (nth_change_dfl W8.zero witness); 1: by rewrite size_state2bytes /= /#.
+by rewrite state2bytesE.
+qed.
+
+lemma derive_commitment_hash_ll : islossless K.__derive_commitment_hash.
+proof.
+proc.
+call A48avx2.dumpstate_avx2_ll.
+call keccakf1600_avx2_ll.
+call A768avx2.absorb_avx2_ll.
+call A64avx2.absorb_avx2_ll.
+call state_init_avx2_ll.
+by auto.
+qed.
+
+phoare derive_commitment_hash_ph' _mu _w1 :
+ [ K.__derive_commitment_hash
+ : arg.`1 = _mu /\ arg.`2 = _w1
+ ==> res = Array48.of_list witness (BytesCT.to_list (H_ct (Bytes64.of_list (to_list _mu)) (BytesW1.of_list (to_list _w1))))
+ ] = 1%r.
+proof.
+by conseq derive_commitment_hash_ll (derive_commitment_hash_h' _mu _w1).
+qed.
 
 phoare derive_commitment_hash_ph _mu _w1 :
  [ M.__derive_commitment_hash
  : arg.`1 = _mu /\ arg.`2 = _w1
  ==> res = Array48.of_list witness (BytesCT.to_list (H_ct (Bytes64.of_list (to_list _mu)) (BytesW1.of_list (to_list _w1))))
  ] = 1%r.
-admitted.
+proof.
+by conseq derive_commitment_hash_eq (derive_commitment_hash_ph' _mu _w1) => // /#.
+qed.
 
-(* __derive_message_representative computes SHAKE256 over:
-     vk_hash (64 bytes) || 0x00 || context_size_byte || context || message
-   which is exactly H_mu(vk_hash, [0x00; context_size_byte] ++ context ++ message).
-   Context and message are read from memory via their pointer/size arguments. *)
+
 phoare derive_message_representative_ph _vk_hash _ctx _msg :
  [ M.__derive_message_representative
  : arg.`1 = _vk_hash /\
@@ -476,4 +723,4 @@ phoare derive_message_representative_ph _vk_hash _ctx _msg :
      (H_mu (Bytes64.of_list (to_list _vk_hash))
            ([W8.zero; truncateu8 (W64.of_int (List.size _ctx))] ++ _ctx ++ _msg)))
  ] = 1%r.
-admitted.
+admitted. (* TODO: NEED MISSING STATEMENTS IN FORMOSA-KECCAK *)
